new take: seccomp -> cminor variant
Here's a variant of the cminor language, called cminorp.  Its main
function takes an input parameter of some memory block.  So only
the initial state differs from the standard Cminor.

The assumption is that the input to Cminorp's main is "correct."

Seccomp.v
@@ -6,6 +6,7 @@ Require Import compcert.common.Values.
 Require Import compcert.lib.Coqlib.
 Require Import compcert.lib.Integers.
 Require Import compcert.lib.Maps.
+Require Import Seccompconf.
 
 Set Implicit Arguments.
 
@@ -87,9 +88,6 @@ Inductive instruction : Type :=
       (** ret A **)
   .
 
-(** sizeof struct seccomp_data *)
-Parameter sizeof_seccomp_data : Z.
-
 Definition code := list instruction.
 
 Section PROGRAM.
@@ -121,6 +119,7 @@ Inductive state : Type :=
     state
   | Callstate:
     forall (fd: fundef)          (**r calling function *)
+           (p: block)            (**r input packet *)
            (m: mem),             (**r memory state *)
     state
   | Returnstate:
@@ -239,21 +238,21 @@ Inductive step (ge: genv) : state -> trace -> state -> Prop :=
       step ge (State a x sm f (Sret_k k :: b) p m)
         E0 (Returnstate k m)
   | exec_call:
-      forall f p m m' m'' bytes,
-      list_length_z bytes = sizeof_seccomp_data ->
-      Mem.alloc m 0 sizeof_seccomp_data = (m', p) ->
-      Mem.storebytes m' p 0 bytes = Some m'' ->
-      step ge (Callstate (Internal f) m)
-        E0 (State Int.zero Int.zero (ZMap.init Int.zero) f f p m')
+      forall f p m,
+      step ge (Callstate (Internal f) p m)
+        E0 (State Int.zero Int.zero (ZMap.init Int.zero) f f p m)
   .
 
 Inductive initial_state (p: program): state -> Prop :=
-  | initial_state_intro: forall b fd m0,
+  | initial_state_intro: forall b fd m0 m1 m2 bytes pkt,
     let ge := Genv.globalenv p in
     Genv.init_mem p = Some m0 ->
     Genv.find_symbol ge p.(prog_main) = Some b ->
     Genv.find_funct_ptr ge b = Some fd ->
-    initial_state p (Callstate fd m0).
+    list_length_z bytes = sizeof_seccomp_data ->
+    Mem.alloc m0 0 sizeof_seccomp_data = (m1, pkt) ->
+    Mem.storebytes m1 pkt 0 bytes = Some m2 ->
+    initial_state p (Callstate fd pkt m2).
 
 Inductive final_state: state -> int -> Prop :=
   | final_state_intro: forall v m,
