Cminorp.v
@@ -1,0 +1,25 @@
+Require Export compcert.backend.Cminor.
+Require Import compcert.common.AST.
+Require Import compcert.common.Globalenvs.
+Require Import compcert.common.Memory.
+Require Import compcert.common.Smallstep.
+Require Import compcert.common.Values.
+Require Import compcert.lib.Coqlib.
+Require Import compcert.lib.Integers.
+Require Import Seccompconf.
+Import ListNotations.
+
+Inductive initial_state (p: Cminor.program): Cminor.state -> Prop :=
+  | initial_state_intro: forall b f m0 m1 m2 bytes pkt,
+      let ge := Genv.globalenv p in
+      Genv.init_mem p = Some m0 ->
+      Genv.find_symbol ge p.(prog_main) = Some b ->
+      Genv.find_funct_ptr ge b = Some f ->
+      funsig f = signature_main ->
+      list_length_z bytes = sizeof_seccomp_data ->
+      Mem.alloc m0 0 sizeof_seccomp_data = (m1, pkt) ->
+      Mem.storebytes m1 pkt 0 bytes = Some m2 ->
+      initial_state p (Callstate f [ Vptr pkt Int.zero ] Kstop m2).
+
+Definition semantics (p: Cminor.program) :=
+  Semantics Cminor.step (initial_state p) Cminor.final_state (Genv.globalenv p).
