Seccompconf.v
@@ -1,0 +1,14 @@
+Require Import compcert.common.AST.
+Require Import compcert.common.Globalenvs.
+Require Import compcert.common.Memory.
+Require Import compcert.common.Smallstep.
+Require Import compcert.common.Values.
+Require Import compcert.lib.Coqlib.
+Require Import compcert.lib.Integers.
+Import ListNotations.
+
+Parameter sizeof_seccomp_data : Z. (**r sizeof struct seccomp_data *)
+
+Definition Tpointer := Tint. (* assume 32-bit pointers *)
+
+Definition signature_main := mksignature [ Tpointer ] (Some Tint) cc_default.
