codegen/extraction.v
@@ -1,6 +1,7 @@
 Require Import ExtrOcamlBasic.
 Require Import ExtrOcamlString.
 Require Import Seccomp.
+Require Import Seccompconf.
 Require Import Seccompjit.
 Require Import Seccompenc.
 Require Import Seccompfilter.
@@ -13,7 +14,7 @@ Extraction Inline Errors.bind Errors.bind2 List.last.
 Extract Constant AST.ident_of_string =>
   "fun s -> Camlcoq.intern_string (Camlcoq.camlstring_of_coqstring s)".
 
-Extract Constant Seccomp.sizeof_seccomp_data =>
+Extract Constant Seccompconf.sizeof_seccomp_data =>
   "Seccompaux.sizeof_seccomp_data".
 
 Extract Constant Seccompjit.seccomp_memwords =>
@@ -21,6 +22,7 @@ Extract Constant Seccompjit.seccomp_memwords =>
 
 Cd "codegen".
 Extraction Library Seccomp.
+Extraction Library Seccompconf.
 Extraction Library Seccompjit.
 Extraction Library Seccompenc.
 Extraction Library Seccompfilter.
